proofs/Lemmas_Replica.dfy
@@ -19,7 +19,7 @@ module M_Lemmas_Replica {
 
     ghost predicate ValidReplicaNextSubSeq(s : seq<ReplicaState>, o : seq<set<Msg>>)
     {
-        && |s| > 2
+        && |s| >= 2
         && |o| == |s| - 1
         && (forall i | 0 <= i < |s| - 1 ::
             && ValidReplicaState(s[i])
@@ -92,7 +92,7 @@ module M_Lemmas_Replica {
             msgReceived := allMsgReceived
         );
         var s : seq<ReplicaState>, o : seq<set<Msg>> :|
-                && |s| > 2
+                && |s| >= 2
                 && |o| == |s| - 1
                 && s[0] == replicaWithNewMsgReceived
                 && s[|s|-1] == r'
@@ -192,7 +192,7 @@ module M_Lemmas_Replica {
             msgReceived := allMsgReceived
         );
         var s : seq<ReplicaState>, o : seq<set<Msg>> :|
-                && |s| > 2
+                && |s| >= 2
                 && |o| == |s| - 1
                 && s[0] == replicaWithNewMsgReceived
                 && s[|s|-1] == r'
@@ -231,7 +231,7 @@ module M_Lemmas_Replica {
             msgReceived := allMsgReceived
         );
         var s : seq<ReplicaState>, o : seq<set<Msg>> :|
-                && |s| > 2
+                && |s| >= 2
                 && |o| == |s| - 1
                 && s[0] == replicaWithNewMsgReceived
                 && s[|s|-1] == r'
@@ -485,7 +485,7 @@ module M_Lemmas_Replica {
             msgReceived := allMsgReceived
         );
         var s : seq<ReplicaState>, o : seq<set<Msg>> :|
-                && |s| > 2
+                && |s| >= 2
                 && |o| == |s| - 1
                 && s[0] == replicaWithNewMsgReceived
                 && s[|s|-1] == r'
